work on prefetch

concurrency/scache/CachePrefetch.i.dfy
@@ -25,6 +25,29 @@ module CacheOps(aio: AIO(CacheAIOParams, CacheIfc, CacheSSM)) {
   import opened LinearSequence_i
   import opened ThreadUtils
   import opened PageSizeConstant
+  import opened IocbStruct
+  import opened GlinearMap
+  import DT = DiskSSMTokens(CacheIfc, CacheSSM)
+  import opened CacheAIOParams
+
+  method get_free_page(shared cache: Cache, linear inout localState: LocalState)
+  returns (
+    cache_idx: uint64,
+    glinear m: T.Token,
+    glinear handle: Handle
+  )
+  requires cache.Inv()
+  requires old_localState.WF()
+  ensures localState.WF()
+  ensures
+      && 0 <= cache_idx as int < CACHE_SIZE as int
+      && m.loc == cache.status[cache_idx].rwlock_loc
+      && m.val == RwLock.ReadHandle(RwLock.ReadPending)
+      && handle.is_handle(cache.key(cache_idx as int))
+      && handle.CacheEmptyHandle?
+  ensures localState.t == old_localState.t
+  decreases *
+
 
   // try to get read lock and immediately release
   // mark access bit on success
@@ -48,7 +71,7 @@ module CacheOps(aio: AIO(CacheAIOParams, CacheIfc, CacheSSM)) {
 
     var is_exc_locked := cache.status_atomic(cache_idx).quicktest_is_exc_locked();
     if is_exc_locked {
-      success := false;
+      in_cache := false;
       client_out := client;
     } else {
       // 2. inc ref
@@ -89,8 +112,61 @@ module CacheOps(aio: AIO(CacheAIOParams, CacheIfc, CacheSSM)) {
         client_out := client';
       }
 
-      success := true;
+      in_cache := true;
     }
+  }
+
+  predicate prefetch_loop_inv(cache: Cache, pages_in_req: int,
+      slot_Idx: int,
+      iocb: Iocb,
+      iovec: PointsToArray<Iovec>,
+      iovec_ptr: Ptr,
+      keys: seq<Key>,
+      cache_readings: map<nat, CacheResources.CacheReading>,
+      idxs: map<nat, CellContents<int64>>,
+      ros: map<nat, T.Token>,
+      wps: map<nat, PointsToArray<byte>>,
+      tickets: map<nat, DT.Token>)
+  {
+    true
+  }
+
+  method prefetch_io(shared cache: Cache, pages_in_req: uint64,
+      addr: uint64,
+      slot_idx: uint64,
+      glinear iocb: Iocb,
+      glinear iovec: PointsToArray<Iovec>,
+      iovec_ptr: Ptr,
+      ghost keys: seq<Key>,
+      glinear cache_readings: map<nat, CacheResources.CacheReading>,
+      glinear idxs: map<nat, CellContents<int64>>,
+      glinear ros: map<nat, T.Token>,
+      glinear wps: map<nat, PointsToArray<byte>>,
+      glinear tickets: map<nat, DT.Token>)
+  requires cache.Inv()
+  requires pages_in_req < addr
+  requires prefetch_loop_inv(cache, pages_in_req as int,
+            slot_idx as int, iocb, iovec, iovec_ptr,
+            keys, cache_readings, idxs, ros, wps, tickets)
+  {
+    glinear var iocb' := iocb;
+    var iocb_ptr := lseq_peek(cache.io_slots, slot_idx).iocb_ptr;
+    iocb_prepare_writev(
+        iocb_ptr,
+        inout iocb',
+        (addr - pages_in_req) as int64,
+        iovec_ptr,
+        pages_in_req);
+
+    glinear var g := ReadvG(keys, cache_readings, idxs, ros, slot_idx as int);
+
+    aio.async_readv(cache.ioctx,
+        iocb_ptr,
+        iocb',
+        iovec,
+        wps,
+        g,
+        tickets);
   }
 
   method prefetch(
@@ -98,7 +174,7 @@ module CacheOps(aio: AIO(CacheAIOParams, CacheIfc, CacheSSM)) {
       inout linear localState: LocalState,
       base_addr: uint64,
       glinear client: Client)
-  returns (client_out: Client)
+  returns (glinear client_out: Client)
   requires cache.Inv()
   requires old_localState.WF()
   requires base_addr % PAGES_PER_EXTENT == 0
@@ -109,24 +185,156 @@ module CacheOps(aio: AIO(CacheAIOParams, CacheIfc, CacheSSM)) {
     client_out := client;
 
     var pages_in_req: uint64 := 0;
+    var slot_idx: uint64 := 0;
+    glinear var iocb_opt : glOption<Iocb> := glNone;
+    glinear var iovec_opt : glOption<PointsToArray<Iovec>> := glNone;
+    var iovec_ptr : Ptr := nullptr();
+
+    ghost var keys: seq<Key> := [];
+    glinear var cache_readings: map<nat, CacheResources.CacheReading> := glmap_empty();
+    glinear var idxs: map<nat, CellContents<int64>> := glmap_empty();
+    glinear var ros: map<nat, T.Token> := glmap_empty();
+    glinear var wps: map<nat, PointsToArray<byte>> := glmap_empty();
+    glinear var tickets: map<nat, DT.Token> := glmap_empty();
 
     var page_off: uint64 := 0;
     while page_off < PAGES_PER_EXTENT
     invariant pages_in_req as int <= page_off as int
+    invariant pages_in_req != 0 ==>
+        && iocb_opt.glSome?
+        && iovec_opt.glSome?
+        && iovec_opt.glSome?
+        && prefetch_loop_inv(cache, pages_in_req as int,
+            slot_idx as int, iocb_opt.value, iovec_opt.value, iovec_ptr,
+            keys, cache_readings, idxs, ros, wps, tickets)
+    decreases *
     {
       var addr := base_addr + page_off;
 
       var cache_idx := atomic_index_lookup_read(
-          cache.cache_idx_of_page_atomic(disk_idx), disk_idx as nat);
+          cache.cache_idx_of_page_atomic(addr), addr as nat);
 
-      var already_in_cache := try_get_and_release(
-          cache, cache_idx, addr as int64, localState, client_out);
+      var already_in_cache;
+      already_in_cache, client_out := try_get_read_and_release(
+          cache, cache_idx, localState, client_out);
 
       if already_in_cache {
         // contiguous chunk of stuff to read in ends here
         // do an I/O request if we have a nonempty range
+        
+        prefetch_io(cache, pages_in_req, addr, slot_idx,
+            unwrap_value(iocb_opt), unwrap_value(iovec_opt),
+            iovec_ptr,
+            keys, cache_readings, idxs, ros, wps, tickets);
+
+        pages_in_req := 0;
+        page_off := page_off + 1;
+
+        keys := [];
+        cache_readings := glmap_empty();
+        idxs := glmap_empty();
+        ros := glmap_empty();
+        wps := glmap_empty();
+        tickets := glmap_empty();
+        iocb_opt := glNone;
+        iovec_opt := glNone;
       } else {
         // append to the current range
+
+        // first, grab a free page:
+
+        glinear var r, handle;
+        var cache_idx;
+        cache_idx, r, handle := get_free_page(cache, inout localState);
+
+        glinear var CacheEmptyHandle(_, cache_empty, idx, wp) := handle;
+
+        glinear var cache_empty_opt, cache_reading_opt, read_ticket_opt;
+        var success;
+        success, cache_empty_opt, cache_reading_opt, read_ticket_opt := 
+            atomic_index_lookup_add_mapping(
+              cache.cache_idx_of_page_atomic(addr),
+              addr,
+              cache_idx,
+              cache_empty);
+
+        if !success {
+          // oops, page is already in cache
+          // release the free page and just try this iteration over again
+          cache.status_atomic(cache_idx).abandon_reading_pending(
+            r,
+            CacheEmptyHandle(
+                cache.key(cache_idx as int),
+                unwrap_value(cache_empty_opt),
+                idx,
+                wp));
+
+          dispose_anything(read_ticket_opt);
+          dispose_anything(cache_reading_opt);
+        } else {
+          write_cell(
+            cache.disk_idx_of_entry_ptr(cache_idx),
+            inout idx,
+            addr as int64);
+
+          if pages_in_req == 0 {
+            glinear var access;
+            var sidx;
+            sidx, access := get_free_io_slot(cache, inout localState);
+            iovec_ptr := lseq_peek(cache.io_slots, sidx).iocb_ptr;
+
+            slot_idx := sidx;
+            glinear var IOSlotAccess(iocb, iovec) := access;
+            dispose_anything(iocb_opt);
+            dispose_anything(iovec_opt);
+            iocb_opt := glSome(iocb);
+            iovec_opt := glSome(iovec);
+          }
+
+          glinear var iovec := unwrap_value(iovec_opt);
+          var iov := new_iovec(cache.data_ptr(cache_idx), 4096);
+          iovec_ptr.index_write(inout iovec, pages_in_req, iov);
+          iovec_opt := glSome(iovec);
+
+          keys := keys + [cache.key(cache_idx as int)];
+          cache_readings := glmap_insert(cache_readings,
+              pages_in_req as int,
+              unwrap_value(cache_reading_opt));
+          idxs := glmap_insert(idxs,
+              pages_in_req as int,
+              idx);
+          ros := glmap_insert(ros,
+              pages_in_req as int,
+              r);
+          wps := glmap_insert(wps,
+              pages_in_req as int,
+              wp);
+          tickets := glmap_insert(tickets,
+              pages_in_req as int,
+              CacheResources.DiskReadTicket_unfold(unwrap_value(read_ticket_opt)));
+
+          dispose_anything(cache_empty_opt);
+
+          pages_in_req := pages_in_req + 1;
+          page_off := page_off + 1;
+        }
       }
     }
+
+    if pages_in_req != 0 {
+      var addr := base_addr + page_off;
+      prefetch_io(cache, pages_in_req, addr, slot_idx,
+          unwrap_value(iocb_opt), unwrap_value(iovec_opt),
+          iovec_ptr,
+          keys, cache_readings, idxs, ros, wps, tickets);
+    } else {
+      dispose_anything(iocb_opt);
+      dispose_anything(iovec_opt);
+      dispose_anything(cache_readings);
+      dispose_anything(idxs);
+      dispose_anything(ros);
+      dispose_anything(wps);
+      dispose_anything(tickets);
+    }
   }
+}
